pointNegate extracted ~ low ~ mid

src/specs/pointNegate.ec
@@ -1,102 +1,39 @@
 pragma Goals:printall.
 
 require import AllCore Int IntDiv Constants Field.
-(* require import Memory PurePrimops UInt256 Utils YulPrimops. *)
+require import Memory PurePrimops UInt256 Utils YulPrimops.
 
-type Point = FieldQ.F * FieldQ.F.
+import FieldQ.
+
+type Point = F * F.
+
+print asint.
 
 pred IsPointValid (point: Point) =
-  !(point.`1 <> zero /\ point.`2 = zero).
+  !(point.`1 <> FieldQ.zero /\ point.`2 = FieldQ.zero).
 
 (* High *)
 op pointNegate (point: Point): Point option =
   if !IsPointValid point then None else Some (point.`1, -(point.`2)).
 
 module PointNegate = {
-  proc usr_pointNegate'(usr_point : uint256): unit = {
-    var _2, usr_pY,  tmp90, tmp91, _6, _7 : uint256;
-    _2 <- (usr_point + W256.of_int 32);
-    usr_pY <@ Primops.mload(_2);
-    if ((usr_pY = (W256.of_int 0)))
-      {
-      tmp90 <@ Primops.mload(usr_point);
-      if (bool_of_uint256 tmp90)
-        {
-        usr_revertWithMessage((W256.of_int 26), PurePrimops.STRING);
-        }
-      }
-    else {
-      Primops.mstore(_2, ((W256.of_int (asint Q)) - usr_pY));
-      }
-    }
 
-  (* proc low(point: uint256) : unit = { *)
-  (*   var x, y; *)
-  (*   x <@ Primops.mload(point); *)
-  (*   y <@ Primops.mload(point + W256.of_int 32); *)
-  (*   if (y <> W256.zero) { *)
-  (*       Primops.mstore(point + W256.of_int 32, p_uint256 - y); *)
-  (*   } *)
-    
-  (*   if (x <> W256.zero /\ y = W256.zero) { *)
-  (*     Primops.revert(W256.zero, W256.zero); *)
-  (*   } *)
-  (* } *)
-
-  proc mid(point_x: int, point_y: int) : int * int = {
-    var ret_x, ret_y;
-    ret_x <- point_x;
-    ret_y <- point_y;
-    if (point_y = 0) {
-      if (point_x <> 0 ){
-        Primops.reverted <- true;
-      }
-    } else {
-        ret_y <- (-point_y) %% p_int;
-    }
-    return (ret_x, ret_y);
+  proc usr_revertWithMessage(usr_len : uint256, usr_reason : uint256): unit = {
+  var _1, _2, _3, _4, _5, _6, _7;
+  _1 <- (PurePrimops.shl (W256.of_int 229) (W256.of_int 4594637));
+  _2 <- (W256.of_int 0);
+  Primops.mstore(_2, _1);
+  _3 <- (W256.of_int 32);
+  _4 <- (W256.of_int 4);
+  Primops.mstore(_4, _3);
+  _5 <- (W256.of_int 36);
+  Primops.mstore(_5, usr_len);
+  _6 <- (W256.of_int 68);
+  Primops.mstore(_6, usr_reason);
+  _7 <- (W256.of_int 100);
+  Primops.revert(_2, _7);
   }
-  
-  (* proc mid(point_x: int, point_y: int) : int * int = { *)
-  (*   var ret_x, ret_y; *)
-  (*   ret_x <- point_x; *)
-  (*   ret_y <- (-point_y) %% p_int; *)
 
-  (*   if (point_x <> 0 /\ point_y = 0) { *)
-  (*     Primops.reverted <- true; *)
-  (*   } *)
-
-  (*   return (ret_x, ret_y); *)
-  (* } *)
-
-  (*     proc high(point: Point): Point = { *)
-  (*   (* option instead of revert *) *)
-  (*   if (!IsPointValid point) { *)
-  (*     Primops.reverted <- true; *)
-  (*   } *)
-
-  (*   return (NegatePoint point); *)
-  (* } *)
-}.
-
-(* DENIS *)
-
-module Test = {
-    proc usr_revertWithMessage(usr_len : uint256, usr_reason : uint256): unit = {
-    var _1, _2, _3, _4, _5, _6, _7;
-    _1 <- (PurePrimops.shl (W256.of_int 229) (W256.of_int 4594637));
-    _2 <- (W256.of_int 0);
-    Primops.mstore(_2, _1);
-    _3 <- (W256.of_int 32);
-    _4 <- (W256.of_int 4);
-    Primops.mstore(_4, _3);
-    _5 <- (W256.of_int 36);
-    Primops.mstore(_5, usr_len);
-    _6 <- (W256.of_int 68);
-    Primops.mstore(_6, usr_reason);
-    _7 <- (W256.of_int 100);
-    Primops.revert(_2, _7);
-    }
   proc usr_pointNegate(usr_point : uint256): unit = {
     var _1, _2, usr_pY, tmp88, tmp89, _3, tmp90, _4, _5, tmp91, _6, _7;
     _1 <- (W256.of_int 32);
@@ -116,36 +53,27 @@ module Test = {
         }
       }
     else {
-      _6 <- (W256.of_int 21888242871839275222246405745257275088696311157297823662689037894645226208583);
+      _6 <- (W256.of_int Q);
       _7 <- (_6 - usr_pY);
       Primops.mstore(_2, _7);
       }
     }
-    proc writeReadTest(address: uint256, value: uint256): uint256 = {
-      var _1;
-      Primops.mstore(address, value);
-      _1 <@ Primops.mload(address);
-      return _1;
-    }
-    
-  proc usr_pointNegate'(usr_point : uint256): unit = {
-    var _2, usr_pY,  tmp90, tmp91, _6, _7 : uint256;
+
+  proc low(usr_point : uint256): unit = {
+    var _2, usr_pY, tmp90, tmp91, _6, _7 : uint256;
     _2 <- (usr_point + W256.of_int 32);
     usr_pY <@ Primops.mload(_2);
-    if ((usr_pY = (W256.of_int 0)))
-      {
+    if ((usr_pY = (W256.of_int 0))) {
       tmp90 <@ Primops.mload(usr_point);
-      if (bool_of_uint256 tmp90)
-        {
+      if (bool_of_uint256 tmp90) {
         usr_revertWithMessage((W256.of_int 26), PurePrimops.STRING);
         }
-      }
-    else {
-      Primops.mstore(_2, ((W256.of_int 21888242871839275222246405745257275088696311157297823662689037894645226208583) - usr_pY));
-      }
     }
+    else {
+      Primops.mstore(_2, ((W256.of_int Q) - usr_pY));
+    }
+  }
 
-    
   proc mid(point_x: int, point_y: int) : int * int = {
     var ret_x, ret_y;
     ret_x <- point_x;
@@ -155,28 +83,29 @@ module Test = {
         Primops.reverted <- true;
       }
     } else {
-        ret_y <- (-point_y) %% p_int;
+      ret_y <- (-point_y) %% Q;
     }
     return (ret_x, ret_y);
   }
-  }.
+}.
 
-
-lemma boring_proof1 : equiv [Test.usr_pointNegate ~ Test.usr_pointNegate' : ={arg, glob Test} ==> ={glob Test} /\ ={res}].
-proc. 
-seq 5  2 : (#pre /\ ={usr_pY, _2} /\ usr_pY{1} = tmp89{1}).
+lemma pointNegate_extracted_equiv_low :
+   equiv [PointNegate.usr_pointNegate ~ PointNegate.low :
+            ={arg, glob PointNegate} ==> ={res}].
+proof.
+proc.
+seq 5 2 : (#pre /\ ={usr_pY, _2} /\ usr_pY{1} = tmp89{1}).
 wp.
-call (_: ={glob Test}). wp. skip. auto.
+call (_: ={glob PointNegate}). wp. skip. auto.
 wp. auto.
 if. auto. 
 inline *. sp. wp.
 skip. auto.
-call (_: ={glob Test}). auto. wp. auto.
+call (_: ={glob PointNegate}). auto. wp. rewrite /Q. auto.
 qed.
 
-lemma boring_proof2 (memory: mem) (point_address: uint256) (point_x_int point_y_int: int): equiv [
-    Test.usr_pointNegate' ~ Test.mid :
-      ={glob Test} /\ (* revise *)
+lemma pointNegate_low_equiv_mid (memory: mem) (point_address: uint256) (point_x_int point_y_int: int): equiv [
+    PointNegate.low ~ PointNegate.mid :
       arg{2} = (point_x_int, point_y_int) /\ arg{1} = point_address /\
       Primops.memory{1} = memory /\
       W256.to_uint(PurePrimops.mload memory point_address) = point_x_int /\
@@ -184,11 +113,24 @@ lemma boring_proof2 (memory: mem) (point_address: uint256) (point_x_int point_y_
       !Primops.reverted{1} /\ !Primops.reverted{2}
       ==>
       Primops.reverted{1} <=> Primops.reverted{2} /\ (
-        (!Primops.reverted{1}) /\ (
+        (!Primops.reverted{1}) => (
           Primops.memory{1} = PurePrimops.mstore (PurePrimops.mstore memory point_address (W256.of_int res{2}.`1)) (point_address + W256.of_int 32) (W256.of_int res{2}.`2)
         )
-            \/
-        (Primops.reverted{1}) /\ ( (* .. *) )
       )
     ].
 proof. proc.
+seq 2 2 : (#pre /\ ret_x{2} = point_x{2} /\ ret_y{2} = point_y{2} /\ W256.to_uint usr_pY{1} = ret_y{2}).
+call {1} (ConcretePrimops.mload_pspec memory (point_address + W256.of_int 32)).
+wp. skip.  auto.
+if. smt (@W256).
+seq 1 0 : (#pre /\ W256.to_uint tmp90{1} = point_x_int{2}).
+exists*  usr_point{1}. elim*. move => usr_point_l.
+call {1} (ConcretePrimops.mload_pspec memory (usr_point_l)). skip. auto.
+if. 
+smt(@W256). inline*. auto. skip. auto.
+simplify.
+exists* _2{1},  usr_pY{1}. elim*. move => _2_l usr_pY_l.
+call {1} (ConcretePrimops.mstore_pspec memory _2_l ((of_int Q)%W256 - usr_pY_l)).
+wp. skip. 
+progress.
+qed.
